\documentclass{beamer}
\usepackage{tikz,amsmath,hyperref,graphicx,stackrel,animate}
\usetikzlibrary{positioning,shadows,arrows,shapes,calc}
\newcommand{\argmax}{\operatornamewithlimits{argmax}}
\newcommand{\argmin}{\operatornamewithlimits{argmin}}
\mode<presentation>{\usetheme{Frankfurt}}
\AtBeginSection[]
{
  \begin{frame}<beamer>
    \frametitle{Outline}
    \tableofcontents[currentsection,currentsubsection]
  \end{frame}
}
\title{Lecture 3: Spectrum}
\author{Mark Hasegawa-Johnson}
\date{ECE 401: Signal and Image Analysis}
\begin{document}

% Title
\begin{frame}
  \maketitle
\end{frame}

% Title
\begin{frame}
  \tableofcontents
\end{frame}

%%%%%%%%%%%%%%%%%%%%%%%%%%%%%%%%%%%%%%%%%%%%
\section[Beating]{Beat Tones}
\setcounter{subsection}{1}

\begin{frame}
  \frametitle{Beat tones}

  When two pure tones at similar frequencies are added together, you hear the  two tones
  ``beating'' against each other.
  \vspace*{1cm}
  \centerline{\fbox{\href{https://en.wikipedia.org/wiki/Beat_(acoustics)}{Beat tones demo}}}
\end{frame}

\begin{frame}
  \frametitle{Beat tones and Trigonometric identities}

  Beat tones can be explained using this trigonometric identity:
  \[
  \cos(a)\cos(b)=\frac{1}{2}\cos(a+b)+\frac{1}{2}\cos(a-b)
  \]
  Let's do the following variable substitution:
  \begin{align*}
    a+b &= 2\pi f_1 t\\
    a-b &= 2\pi f_2 t\\
    a &= 2\pi f_{ave}t\\
    b &= 2\pi f_{beat}t
  \end{align*}
  where $f_{ave}=\frac{f_1+f_2}{2}$, and $f_{beat}=\frac{f_1-f_2}{2}$.
\end{frame}

\begin{frame}
  \frametitle{Beat tones and Trigonometric identities}

  Re-writing the trigonometric identity, we get:
  \[
  \frac{1}{2}\cos(2\pi f_1t)+\frac{1}{2}\cos(2\pi f_2 t) = \cos(2\pi f_{beat}t)\cos(2\pi f_{ave}t)
  \]
  So when we play two tones together, $f_1=110$Hz and $f_2=104$Hz, it
  sounds like we're playing a single tone at $f_{ave}=107$Hz,
  multiplied by a beat frequency $f_{beat}=3$ (double beats)/second.
\end{frame}

\begin{frame}
  \frametitle{Beat tones\\\begin{tiny}by Adjwilley, CC-SA 3.0,
    \url{https://commons.wikimedia.org/wiki/File:WaveInterference.gif}\end{tiny}}
  \centerline{\animategraphics[loop,controls,width=\textwidth]{20}{exp/WaveInterference-}{0}{80}}
\end{frame}

\begin{frame}
  \frametitle{More complex beat tones}

  What happens if we add together, say, three tones?
  \[
  \cos(2\pi 107t) + \cos(2\pi 110t)+\cos(2\pi 104t)=\mbox{???}
  \]
  For this, and other more complicated operations, it
  is much, much easier to work with complex exponentials, instead of cosines.
\end{frame}
  

\begin{frame}
  \frametitle{More complex beat tones}

  What happens if we add together, say, three tones?
  \[
  x(t) = \cos(2\pi 107t) + \cos(2\pi 110t)+\cos(2\pi 104t)=\mbox{???}
  \]
  This is like a phasor example, except that all of the tones are at
  different frequencies.
  \begin{align*}
    x(t) &= \Re\left\{e^{j2\pi 107t}+e^{j2\pi 110t}+e^{j2\pi 104t}\right\}\\
    &= \Re\left\{\left(1+e^{j2\pi 3t}+e^{-j2\pi 3t}\right)e^{j2\pi 107t}\right\}
  \end{align*}
  So we just have to do this phasor addition:
  \[
  1+e^{j2\pi 3t}+e^{-j2\pi 3t} = 1 + 2\cos\left(2\pi 3t\right)
  \]
\end{frame}

\begin{frame}
  \frametitle{Triple-beat example}

  \centerline{\includegraphics[height=3in]{exp/triplebeat.png}}
\end{frame}

%%%%%%%%%%%%%%%%%%%%%%%%%%%%%%%%%%%%%%%%%%%%
\section[Spectrum]{Spectrum}
\setcounter{subsection}{1}

\begin{frame}
  \frametitle{Phasor representation of a general sum of sinusoids}

  In general, if $x(t)$ is a sum of sines and cosines,
  \[
  x(t) = A_0 + \sum_{k=1}^N A_k\cos\left(2\pi f_kt+\theta_k\right)
  \]
  Then it has a phasor notation
  \[
  x(t) = A_0+\sum_{k=1}^N\Re\left\{A_ke^{j\theta_k}e^{j2\pi f_kt}\right\}
  \]
\end{frame}

\begin{frame}
  \frametitle{Two-sided spectrum}

  The $\Re\left\{z\right\}$ operator is annoying.  In order to get rid
  of it, let's take advantage of Euler's formula
  $\Re\left\{z\right\}=\frac{1}{2}(z+z^*)$ to write:
  \begin{align*}
    x(t) &= A_0+ \sum_{k=1}^N A_k\cos\left(2\pi f_kt+\theta_k\right)\\
    &= \sum_{k=-N}^N a_k e^{j2\pi f_k t}    
  \end{align*}
  In order to do that, we need to define $a_k$ like this:
  \[
  a_k = \begin{cases}
    A_0 & k=0\\
    \frac{1}{2}A_ke^{j\theta_k} & k>0\\
    \frac{1}{2}A_{-k}e^{-j\theta_{-k}} & k < 0
  \end{cases}
  \]  
\end{frame}

\begin{frame}
  \frametitle{Two-sided spectrum}

  The {\bf spectrum} of $x(t)$ is the set of frequencies, and their
  associated phasors,
  \[
  \mbox{Spectrum}\left( x(t) \right) =
  \left\{ (f_{-N},a_{-N}), \ldots, (f_0,a_0), \ldots, (f_N,a_N) \right\}
  \]
  such that
  \[
  x(t) = \sum_{k=-N}^N a_ke^{j2\pi f_kt}
  \]
\end{frame}

\begin{frame}
  \frametitle{Quiz}

  Try the quiz!  Go to the course webpage, and click on today's date to try the quiz.
\end{frame}

%%%%%%%%%%%%%%%%%%%%%%%%%%%%%%%%%%%%%%%%%%%%
\section[Properties]{Properties of a Spectrum}
\setcounter{subsection}{1}

\begin{frame}
  \frametitle{Properties of a spectrum}

  Spectrum representation is nice to use because
  \begin{itemize}
  \item It's so general.  Any signal made up of pure tones can be written this way.
  \item Many signal processing operations can be written directly in
    the spectral domain (as operations on $a_k$), without converting
    back to $x(t)$.
  \end{itemize}
\end{frame}

\begin{frame}
  \frametitle{Property \#1: Scaling}

  Suppose we have a signal
  \[
  x(t) = \sum_{k=-N}^N a_ke^{j2\pi f_kt}
  \]
  Suppose we scale it by a factor of $G$:
  \[
  y(t) = Gx(t)
  \]
  That just means that we scale each of the coefficients by $G$:
  \[
  y(t)  = \sum_{k=-N}^N \left(Ga_k\right) e^{j2\pi f_kt}
  \]
\end{frame}

\begin{frame}
  \frametitle{Property \#2: Adding a constant}

  Suppose we have a signal
  \[
  x(t) = \sum_{k=-N}^N a_ke^{j2\pi f_kt}
  \]
  Suppose we add a constant, $C$:
  \[
  y(t) = x(t) + C
  \]
  That just means that we add that constant to $a_0$:
  \[
  y(t)  = (a_0+C) + \sum_{k\ne 0} a_k e^{j2\pi f_kt}
  \]
\end{frame}

\begin{frame}
  \frametitle{Property \#3: Adding two signals}

  Suppose we have two signals:
  \begin{align*}
    x(t) &= \sum_{n=-N}^N a_n'e^{j2\pi f_n't}\\
    y(t) &= \sum_{m=-M}^M a_m''e^{j2\pi f_m''t}
  \end{align*}
  and we add them together:
  \[
  z(t) = x(t) + y(t) = \sum_k a_ke^{j2\pi f_kt}
  \]
  where, if a frequency $f_k$ comes from both $x(t)$ and $y(t)$, then
  we have to do phasor addition:
  \[
  \mbox{If}~f_k=f_n'=f_m''~~\mbox{then}~~a_k=a_n'+a_m''
  \]
\end{frame}

\begin{frame}
  \frametitle{Property \#4: Time shift}

  Suppose we have a signal
  \[
  x(t) = \sum_{k=-N}^N a_ke^{j2\pi f_kt}
  \]
  and we want to time shift it by $\tau$ seconds:
  \[
  y(t) = x(t-\tau)
  \]
  Time shift corresponds to a {\em\bf phase shift} of each spectral component:
  \[
  y(t) = \sum_{k=-N}^N \left(a_ke^{-j2\pi f_k\tau}\right)e^{j2\pi f_kt}
  \]
\end{frame}

\begin{frame}
  \frametitle{Property \#5: Frequency shift}

  Suppose we have a signal
  \[
  x(t) = \sum_{k=-N}^N a_ke^{j2\pi f_kt}
  \]
  and we want to shift it in frequency by some constant overall shift, $F$:
  \[
  y(t) = \sum_{k=-N}^N a_ke^{j2\pi \left(f_k+F\right)t}
  \]
  Frequency shift corresponds to amplitude modulation (multiplying it by a
  complex exponential at the carrier frequency $F$):
  \[
  y(t) = x(t) e^{j2\pi Ft}
  \]
\end{frame}

\begin{frame}
  \frametitle{Property \#6: Differentiation}

  Suppose we have a signal
  \[
  x(t) = \sum_{k=-N}^N a_ke^{j2\pi f_kt}
  \]
  and we want to differentiate it:
  \[
  y(t) \propto \frac{dx}{dt}
  \]
  Differentiation corresponds to scaling each spectral coefficient by
  $j2\pi f_k$:
  \[
  y(t) = \sum_{k=-N}^N \left(j2\pi f_k a_k\right)e^{j2\pi f_kt}
  \]
\end{frame}


%%%%%%%%%%%%%%%%%%%%%%%%%%%%%%%%%%%%%%%%%%%%
\section[Spectrum of Beat Tones]{Spectrum of Beat Tones}
\setcounter{subsection}{1}

\begin{frame}
  \frametitle{Representing beat tones with no trig identities}

  One nice thing about the spectral representation is that you can
  analyze beat tones without remembering any trig identities.

  First, write out the spectrum:
  \begin{displaymath}
    2\cos(2\pi f_1t)+2\cos(2\pi f_2t)=
    e^{-j2\pi f_2t}+e^{-j2\pi f_1t}+e^{j2\pi f_1t}+e^{j2\pi f_2t}
  \end{displaymath}
\end{frame}

\begin{frame}
  \frametitle{Representing beat tones with no trig identities}

  Second, write the spectrum in terms of the carrier frequency
  $f_c=\frac{f_2+f_1}{2}$ and the beat frequency
  $f_b=\frac{f_2-f_1}{2}$:

  \begin{displaymath}
    e^{-j2\pi f_2t}+e^{-j2\pi f_1t}+e^{j2\pi f_1t}+e^{j2\pi f_2t} =
    e^{-j2\pi (f_c+b_b)t}+e^{-j2\pi (f_c-f_b)t}+e^{j2\pi (f_c-f_b)t}+e^{j2\pi (f_c+f_b)t}
  \end{displaymath}
\end{frame}

\begin{frame}
  \frametitle{Representing beat tones with no trig identities}

  Third, remember that $xy+xz=x(y+z)$, so

  \begin{displaymath}
    e^{-j2\pi (f_c+b_b)t}+e^{-j2\pi (f_c-f_b)t}+e^{j2\pi (f_c-f_b)t}+e^{j2\pi (f_c+f_b)t}=
    \left(e^{-j2\pi f_bt}+e^{j2\pi f_bt}\right)\left(e^{-j2\pi f_ct}+e^{j2\pi f_ct}\right)=
    4\cos\left(2\pi f_bt\right)\cos\left(2\pi f_c\right)
  \end{displaymath}
\end{frame}

\begin{frame}
  \frametitle{Representing beat tones with no trig identities}

  Solving for beat tones using the spectrum took longer than using a
  trig identity, but it has the key advantage that we didn't have to
  remember any trig identity.  The result is the same, but we can do
  it even when we don't have an internet connection.
  
  \[
  2\cos(2\pi f_1t)+2\cos(2\pi f_2 t) = 4\cos(2\pi f_{b}t)\cos(2\pi f_{c}t)
  \]
\end{frame}


%%%%%%%%%%%%%%%%%%%%%%%%%%%%%%%%%%%%%%%%%%%%
\section[Summary]{Summary}
\setcounter{subsection}{1}

\begin{frame}
  \frametitle{Summary}
  \begin{itemize}
  \item {\bf Spectrum:} The spectrum of any sum of cosines is the set
    of complex-valued spectral coefficients, $a_k$, matched with the
    frequencies $f_k$, such that
    \[
    x(t) = \sum_{k=-N}^N a_ke^{j2\pi f_kt}
    \]
  \item {\bf Properties of the spectrum:} signal processing operations
    that can be done directly in the spectrum, without first
    recomputing the waveform, include scaling, adding, time shift,
    frequency shift, and differentiation.
  \end{itemize}
  
\end{frame}

\end{document}
